Com - 副本.thy
@@ -1,0 +1,12 @@
+section "ReqCom --- The Commmand of Regrexp Expressions"
+
+theory Com imports Areg begin
+
+datatype 'a com = SKIP 
+      | Match "'a option"  "'a option regexp" nat        
+      | Search "'a option regexp" "'a option" nat       
+      | Replace "'a option regexp" "'a option" "'a option"     
+      | Split "'a option regexp" "'a option" "'a option list"    
+      | Extract "'a option" nat 
+
+end
